blockDAG_Type.thy
@@ -3,31 +3,251 @@
 *)
 
 theory blockDAG_Type      
-  imports blockDAG 
+  imports blockDAG Spectre Codegen
 begin
 
-typedef ('a,'b) BlockDAG = "{x. blockDAG x}::('a,'b) pre_digraph set"
-  morphisms BlockDAG pre_digraph_ext
-proof
-  fix a::'a
-  let ?x = "\<lparr>verts = {a}, arcs = {}, tail = \<lambda>x. a, head =  \<lambda>x. a\<rparr>" 
-  have "blockDAG ?x" unfolding blockDAG_def blockDAG_axioms_def DAG_def DAG_axioms_def 
+locale  simp_pre_digraph = 
+  fixes G::"('a,'a \<times> 'a) pre_digraph"
+  assumes tail_fst: "tail G = fst"
+  and head_snd: "head G = snd"
+
+locale simp_digraph = simp_pre_digraph + 
+  assumes "digraph G"
+
+locale simp_blockDAG =
+  simp_pre_digraph  + 
+  assumes bD: "blockDAG G"
+
+sublocale simp_pre_digraph \<subseteq> pre_digraph .
+
+sublocale simp_blockDAG \<subseteq> blockDAG using bD by simp
+
+lemma ssubs: "simp_blockDAG G \<Longrightarrow> blockDAG G" using simp_blockDAG.bD by auto
+
+
+definition empty_graph :: "('a,'a \<times> 'a) pre_digraph" 
+  where "empty_graph = \<lparr>verts = {}, arcs = {}, tail = fst, head =  snd\<rparr>"
+
+global_interpretation  simp_digraph empty_graph 
+  unfolding simp_digraph_def simp_pre_digraph_def simp_digraph_axioms_def
+    digraph_def fin_digraph_def wf_digraph_def  empty_graph_def
+  fin_digraph_axioms_def loopfree_digraph_def loopfree_digraph_axioms_def nomulti_digraph_def
+  nomulti_digraph_axioms_def by force
+  
+
+fun balance_BD :: "('a,'a \<times> 'a) pre_digraph \<Rightarrow> ('a,'a \<times> 'a) pre_digraph"
+  where "balance_BD G = (if (simp_blockDAG G) then G else empty_graph)"
+
+
+text \<open>Rewrite to get better performance (including base subgraph inducing)\<close>
+definition reduce_past_empty:: "('a,'a \<times> 'a) pre_digraph \<Rightarrow> 'a \<Rightarrow> ('a,'a \<times> 'a) pre_digraph"
+  where "reduce_past_empty G a = balance_BD (reduce_past G a)"
+
+definition some_genesis :: "'a \<Rightarrow> ('a,'b) pre_digraph" 
+  where "some_genesis a = \<lparr>verts = {a}, arcs = {}, tail = \<lambda>x. a, head =  \<lambda>x. a\<rparr>"
+
+lemma some_bD:  "blockDAG (some_genesis a)"
+unfolding some_genesis_def blockDAG_def blockDAG_axioms_def DAG_def DAG_axioms_def 
   digraph_def loopfree_digraph_def loopfree_digraph_axioms_def nomulti_digraph_def 
   nomulti_digraph_axioms_def wf_digraph_def fin_digraph_def fin_digraph_axioms_def 
   pre_digraph.del_arc_simps
   proof(safe,simp_all, simp add: arcs_ends_def)
     fix u::'a fix  v::'a fix e::'d
-    have "\<not>  u \<rightarrow>\<^sup>+\<^bsub>pre_digraph.del_arc ?x e\<^esub> v " 
+    have "\<not>  u \<rightarrow>\<^sup>+\<^bsub>pre_digraph.del_arc (some_genesis a) e\<^esub> v " 
+      unfolding some_genesis_def
       by (simp add: arcs_ends_def pre_digraph.del_arc_in) 
-    then show "u \<rightarrow>\<^sup>+\<^bsub>pre_digraph.del_arc ?x e\<^esub> v 
-    \<Longrightarrow> wf_digraph.arc ?x e (u, v) \<Longrightarrow> False" by auto
+    then show "wf_digraph.arc \<lparr>verts = {a}, arcs = {}, tail = \<lambda>x. a, head = \<lambda>x. a\<rparr> e (u, v) \<Longrightarrow>
+       u \<rightarrow>\<^sup>+\<^bsub>pre_digraph.del_arc \<lparr>verts = {a}, arcs = {}, tail = \<lambda>x. a, head = \<lambda>x. a\<rparr> e\<^esub> v \<Longrightarrow> False"
+      unfolding some_genesis_def by auto
   qed
-  then show "?x \<in> {x. blockDAG x}" by simp
+
+typedef 'a BlockDAG = "{x. simp_blockDAG x \<or> x = empty_graph}::('a,'a \<times> 'a) pre_digraph set"
+  morphisms pre_digraph_of_BlockDAG Abs_BlockDAG 
+proof
+  show "empty_graph \<in> {x. simp_blockDAG x \<or> x = empty_graph}" by simp
 qed
 
-declare [[coercion BlockDAG]]
+declare [[coercion BlockDAG.pre_digraph_of_BlockDAG]]
 
-lemma
-  "blockDAG (A::('a,'b) BlockDAG)" using BlockDAG by auto
+lemma BD_cases:
+  obtains "simp_blockDAG ((A::'a BlockDAG))" 
+  | "empty_graph =  (A::'a BlockDAG) "
+  using pre_digraph_of_BlockDAG  by fastforce 
 
+setup_lifting BlockDAG.type_definition_BlockDAG 
+context begin
+
+qualified definition abs_BlockDAG :: "('a,'a \<times> 'a) pre_digraph \<Rightarrow> 'a BlockDAG"
+  where "abs_BlockDAG = Abs_BlockDAG o balance_BD"
+
+qualified definition BlockDAG_eq where "BlockDAG_eq = BNF_Def.vimage2p balance_BD balance_BD (=)"
+
+qualified lemma equivp_dlist_eq: "equivp BlockDAG_eq"
+  unfolding BlockDAG_eq_def by(rule equivp_vimage2p)(rule identity_equivp)
+
+definition qcr_BlockDAG :: "('a,'a \<times> 'a) pre_digraph \<Rightarrow> 'a BlockDAG \<Rightarrow> bool" 
+  where "qcr_BlockDAG x y \<longleftrightarrow> y = abs_BlockDAG x"
+
+qualified lemma Quotient_dlist_remdups: "Quotient BlockDAG_eq abs_BlockDAG pre_digraph_of_BlockDAG qcr_BlockDAG"
+  unfolding Quotient_def BlockDAG_eq_def qcr_BlockDAG_def vimage2p_def abs_BlockDAG_def
+proof (auto simp add: fun_eq_iff Abs_BlockDAG_inject
+    pre_digraph_of_BlockDAG[simplified] pre_digraph_of_BlockDAG_inverse)
+  fix a ::"'a  BlockDAG" 
+  assume "\<not> simp_blockDAG (pre_digraph_of_BlockDAG a)"
+  thus "Abs_BlockDAG empty_graph = a"
+    by (metis BD_cases pre_digraph_of_BlockDAG_inverse)
+qed
+    
+end
+lift_definition past_nodes :: " ('a) BlockDAG  \<Rightarrow> 'a \<Rightarrow> 'a set"
+is "DAGs.past_nodes" .
+
+lift_definition reduce_past :: " ('a) BlockDAG  \<Rightarrow> 'a \<Rightarrow> ('a) BlockDAG"
+is "reduce_past_empty" 
+  unfolding reduce_past_empty_def balance_BD.simps by auto
+
+lemma (in simp_blockDAG) simp_blockDAG_reduce_sound:
+  assumes "\<not> is_genesis_node a"
+  and "a \<in> verts G"
+shows "simp_blockDAG (DAGs.reduce_past G a)"
+  unfolding simp_blockDAG_def simp_blockDAG_axioms_def simp_pre_digraph_def
+proof safe 
+  show "blockDAG (DAGs.reduce_past G a)" using assms reduce_past_dagbased  by auto
+  show  "tail (DAGs.reduce_past G a) = fst" 
+    unfolding DAGs.reduce_past.simps using tail_fst induce_subgraph_tail by auto
+  show  "head (DAGs.reduce_past G a) = snd" 
+    unfolding DAGs.reduce_past.simps using head_snd induce_subgraph_head by auto
+qed
+
+lemma (in simp_blockDAG) reduce_lifted_sound:
+  assumes "a \<in> verts G"
+  and "\<not> is_genesis_node a"
+  shows "reduce_past_empty G a = DAGs.reduce_past G a"
+  unfolding reduce_past_empty_def balance_BD.simps 
+  using assms simp_blockDAG_reduce_sound by auto
+ 
+  
+
+lift_definition  vote_Spectre_typed  :: "('a::linorder) BlockDAG  \<Rightarrow> 'a \<Rightarrow> 'a \<Rightarrow> 'a \<Rightarrow> int"
+is "Spectre.vote_Spectre".
+
+lift_definition empty_graph_typed :: "('a) BlockDAG"
+is "blockDAG_Type.empty_graph" by simp
+
+lemma vote_Spectre_typed_eq: "vote_Spectre_typed G a b c = vote_Spectre G a b c"
+  by (simp add: vote_Spectre_typed.rep_eq)  
+
+
+lemma empty_no_bD: "\<not> blockDAG empty_graph_typed" 
+  unfolding empty_graph_typed_def empty_graph_def
+  by (metis blockDAG.genesis_in_verts empty_graph_def
+ empty_graph_typed.abs_eq empty_graph_typed.rep_eq empty_iff pre_digraph.select_convs(1))
+
+lemma  empty_no_sbD: "\<not> simp_blockDAG empty_graph_typed" 
+  unfolding simp_blockDAG_def simp_blockDAG_axioms_def using empty_no_bD by auto
+
+lemma BD_head: 
+  fixes G:: "'a BlockDAG"
+  shows "head G = snd"
+  by (metis BD_cases simp_blockDAG.axioms(1) simp_pre_digraph.head_snd simp_pre_digraph_axioms)
+  
+lemma BD_tail: 
+  fixes G:: "'a BlockDAG"
+  shows "tail G = fst"
+  by (metis BD_cases simp_blockDAG.axioms(1) simp_pre_digraph.tail_fst simp_pre_digraph_axioms)
+
+lemma blockDAG_simp:
+  fixes G:: "'a BlockDAG"
+  shows "blockDAG G \<longleftrightarrow> simp_blockDAG G"
+  unfolding simp_blockDAG_def simp_blockDAG_axioms_def simp_pre_digraph_def
+  using BD_head BD_tail by auto
+
+lemma empty_eq_nbD: 
+  "G = empty_graph_typed \<longleftrightarrow> \<not> blockDAG G"
+  using blockDAG_simp empty_no_sbD BD_cases pre_digraph_of_BlockDAG_inject
+  by metis 
+  
+
+lemma vote_Spectre_typed_code [code] : "vote_Spectre_typed G a b c = (
+  if (G = empty_graph_typed \<or> a \<notin> verts  G \<or> b \<notin> verts G \<or> c \<notin> verts G)
+ then 0 else 
+  if (b=c)  then 1 else 
+  if (((a \<rightarrow>\<^sup>+\<^bsub>G\<^esub> b) \<or> a = b) \<and> \<not>(a \<rightarrow>\<^sup>+\<^bsub>G\<^esub> c)) then 1  else
+  if (((a \<rightarrow>\<^sup>+\<^bsub>G\<^esub> c) \<or> a = c) \<and> \<not>(a \<rightarrow>\<^sup>+\<^bsub>G\<^esub> b)) then -1 else
+  if ((a \<rightarrow>\<^sup>+\<^bsub>G\<^esub> b) \<and> (a \<rightarrow>\<^sup>+\<^bsub>G\<^esub> c)) then 
+   (tie_break_int b c (signum (sum_list (map (\<lambda>i.
+ (vote_Spectre_typed (reduce_past G a) i b c)) (sorted_list_of_set (past_nodes G a))))))
+ else 
+   signum (sum_list (map (\<lambda>i.
+   (vote_Spectre_typed G i b c)) (sorted_list_of_set (future_nodes G a)))))" 
+proof(induct "pre_digraph_of_BlockDAG G" a b c rule: vote_Spectre.induct)
+  case (1 a b c)
+  then show ?case 
+proof(cases a b c "pre_digraph_of_BlockDAG G" rule: Spectre_casesAlt)
+  case no_bD
+  then show ?thesis
+    unfolding vote_Spectre_typed_eq empty_eq_nbD
+    by fastforce 
+next
+case equal
+  then show ?thesis unfolding vote_Spectre_typed_eq empty_eq_nbD by simp
+next
+  case one
+  then show ?thesis  unfolding vote_Spectre_typed_eq empty_eq_nbD
+    by simp 
+next
+  case two
+  then show ?thesis unfolding vote_Spectre_typed_eq empty_eq_nbD
+    by auto
+next
+  case three
+  then interpret bD: blockDAG "(pre_digraph_of_BlockDAG G)" by auto
+  have "\<not> blockDAG.is_genesis_node (pre_digraph_of_BlockDAG G) a" 
+    using bD.genesis_reaches_nothing three by auto
+  then have rrr: "reduce_past_empty (pre_digraph_of_BlockDAG G) a
+   = DAGs.reduce_past (pre_digraph_of_BlockDAG G) a" using three 
+    by (simp add: simp_blockDAG.reduce_lifted_sound blockDAG_simp) 
+  show ?thesis unfolding vote_Spectre_typed_eq empty_eq_nbD reduce_past.rep_eq rrr
+  past_nodes.rep_eq
+      using  three
+      by simp        
+next
+  case four
+  show ?thesis unfolding vote_Spectre_typed_eq empty_eq_nbD 
+    by (simp add: 1 four vote_Spectre.elims) 
+qed
+qed
+
+
+
+instantiation BlockDAG :: (type) equal 
+begin
+definition  equal_BlockDAG ::"'a BlockDAG \<Rightarrow> 'a BlockDAG \<Rightarrow> bool" 
+  where " equal_BlockDAG B1 B2 = (
+ (verts B1 =  verts B2) \<and>  (arcs B1 =   arcs B2))
+ "
+
+instance proof
+  fix x y ::"'a BlockDAG"
+  show "equal_class.equal x y = (x = y)" unfolding equal_BlockDAG_def 
+    using pre_digraph_of_BlockDAG_inject BD_head BD_tail
+    by (metis (full_types) old.unit.exhaust pre_digraph.equality)  
+qed
+
+
+
+end
+
+declare equal_BlockDAG_def [code]
+declare simp_pre_digraph_def [code]
+declare simp_blockDAG_axioms_def [code]
+declare simp_blockDAG_def [code]
+
+lift_definition vote_Spectre_typed_FV ::
+ "FV BlockDAG \<Rightarrow> FV \<Rightarrow> FV \<Rightarrow> FV \<Rightarrow> integer"
+  is "(\<lambda>G a b c. integer_of_int (vote_Spectre_typed G a b c))".
+
+export_code  top_sort anticone set blockDAG pre_digraph_ext snd fst vote_Spectre_Int
+ SpectreOrder_Int OrderDAG_Int vote_Spectre_typed_FV  in Haskell module_name BD
+file "code/"
 end
