Spectre_Properties.thy
@@ -12,9 +12,9 @@ lemma vote_Spectre_Preserving:
   shows "vote_Spectre G a b c \<in> {0,1}"
   using assms
 proof(induction G a b c rule: vote_Spectre.induct)
-  case (1 V a b c)
+  case (1 G a b c)
   then show ?case 
-  proof(cases a b c V rule:Spectre_casesAlt)
+  proof(cases a b c G rule:Spectre_casesAlt)
     case no_bD
     then show ?thesis by auto
   next
@@ -29,30 +29,30 @@ proof(induction G a b c rule: vote_Spectre.induct)
       by (metis "local.1.prems" trancl_trans) 
   next
     case three
-    then have a_not_gen: "\<not> blockDAG.is_genesis_node V a"
+    then have a_not_gen: "\<not> blockDAG.is_genesis_node G a"
       using blockDAG.genesis_reaches_nothing
       by metis
-    then have bD: "blockDAG (reduce_past V a)" using blockDAG.reduce_past_dagbased 
+    then have bD: "blockDAG (reduce_past G a)" using blockDAG.reduce_past_dagbased 
         three by auto
-    have b_in2: "b \<in> past_nodes V a" using three by auto
-    also have c_in2: "c \<in> past_nodes V a" using three by auto
-    ultimately have "c \<rightarrow>\<^sup>+\<^bsub>reduce_past V a\<^esub> b" using DAG.reduce_past_path2 three 1
+    have b_in2: "b \<in> past_nodes G a" using three by auto
+    also have c_in2: "c \<in> past_nodes G a" using three by auto
+    ultimately have "c \<rightarrow>\<^sup>+\<^bsub>reduce_past G a\<^esub> b" using DAG.reduce_past_path2 three 1
       by (metis blockDAG.axioms(1)) 
-    then have allsorted01:"\<forall>x. x \<in> set (sorted_list_of_set (past_nodes V a)) \<longrightarrow>
-          vote_Spectre (reduce_past V a) x b c \<in> {0, 1}" using 1 three by auto
-    then have all01: "\<forall>x. x \<in> (past_nodes V a) \<longrightarrow>
-          vote_Spectre (reduce_past V a) x b c \<in> {0, 1}"
-      using  subs three sorted_list_of_set(1) DAG.finite_past
+    then have allsorted01:"\<forall>x. x \<in> set (sorted_list_of_set (past_nodes G a)) \<longrightarrow>
+          vote_Spectre (reduce_past G a) x b c \<in> {0, 1}" using 1 three by auto
+    then have all01: "\<forall>x. x \<in> (past_nodes G a) \<longrightarrow>
+          vote_Spectre (reduce_past G a) x b c \<in> {0, 1}"
+      using  subs(1) three sorted_list_of_set(1) DAG.finite_past
       by metis 
-    obtain wit where wit_in: "wit \<in> past_nodes V a" 
-      and wit_vote: "vote_Spectre (reduce_past V a) wit b c \<noteq> 0"
+    obtain wit where wit_in: "wit \<in> past_nodes G a" 
+      and wit_vote: "vote_Spectre (reduce_past G a) wit b c \<noteq> 0"
       using vote_Spectre_one_exists b_in2 c_in2 bD induce_subgraph_verts reduce_past.simps
       by metis 
-    then have wit_vote1: "vote_Spectre (reduce_past V a) wit b c = 1" using all01
+    then have wit_vote1: "vote_Spectre (reduce_past G a) wit b c = 1" using all01
       by blast 
     obtain the_map where the_map_in: 
-      "the_map = (map (\<lambda>i. vote_Spectre (reduce_past V a) i b c) 
-               (sorted_list_of_set (past_nodes V a)))"
+      "the_map = (map (\<lambda>i. vote_Spectre (reduce_past G a) i b c) 
+               (sorted_list_of_set (past_nodes G a)))"
       by auto  
     have all01_1: "\<forall>x \<in> set the_map. x \<in> {0,1}"
       unfolding the_map_in set_map 
@@ -60,7 +60,7 @@ proof(induction G a b c rule: vote_Spectre.induct)
     have "\<exists>x \<in> set the_map. x = 1"
       unfolding the_map_in set_map 
       using wit_in wit_vote1
-        sorted_list_of_set(1) DAG.finite_past bD subs
+        sorted_list_of_set(1) DAG.finite_past bD subs(1)
       by (metis (no_types, lifting) image_iff three) 
     then have "\<exists>x \<in> set the_map. x > 0"
       using zero_less_one by blast 
@@ -69,29 +69,29 @@ proof(induction G a b c rule: vote_Spectre.induct)
     ultimately have "signum (sum_list the_map) = 1" using sumlist_one_mono by simp
     then have "tie_break_int b c (signum (sum_list the_map)) = 1" using tie_break_int.simps
       by simp
-    then have "vote_Spectre V a b c = 1 " unfolding the_map_in using three vote_Spectre.simps
+    then have "vote_Spectre G a b c = 1 " unfolding the_map_in using three vote_Spectre.simps
       by simp
     then show ?thesis by simp
   next
     case four 
-    then have all01: "\<forall>a2. a2 \<in> set (sorted_list_of_set (future_nodes V a)) \<longrightarrow>
-                              vote_Spectre V a2 b c \<in> {0,1}"
+    then have all01: "\<forall>a2. a2 \<in> set (sorted_list_of_set (future_nodes G a)) \<longrightarrow>
+                              vote_Spectre G a2 b c \<in> {0,1}"
       using 1
       by metis
-    have "\<forall>a2. a2 \<in> set (sorted_list_of_set (future_nodes V a)) 
-                \<longrightarrow> vote_Spectre V a2 b c \<ge> 0" 
+    have "\<forall>a2. a2 \<in> set (sorted_list_of_set (future_nodes G a)) 
+                \<longrightarrow> vote_Spectre G a2 b c \<ge> 0" 
     proof safe
       fix a2
-      assume " a2 \<in> set (sorted_list_of_set (future_nodes V a))"
-      then have "vote_Spectre V a2 b c \<in> {0, 1}" using all01 by auto
-      then show "vote_Spectre V a2 b c  \<ge> 0"
+      assume " a2 \<in> set (sorted_list_of_set (future_nodes G a))"
+      then have "vote_Spectre G a2 b c \<in> {0, 1}" using all01 by auto
+      then show "vote_Spectre G a2 b c  \<ge> 0"
         by fastforce
     qed 
-    then have "(sum_list (map (\<lambda>i. vote_Spectre V i b c) 
-      (sorted_list_of_set (future_nodes V a)))) \<ge> 0" using sum_list_mono sum_list_0
+    then have "(sum_list (map (\<lambda>i. vote_Spectre G i b c) 
+      (sorted_list_of_set (future_nodes G a)))) \<ge> 0" using sum_list_mono sum_list_0
       by metis 
-    then have "signum (sum_list (map (\<lambda>i. vote_Spectre V i b c) 
-      (sorted_list_of_set (future_nodes V a)))) \<in> {0,1}" unfolding signum.simps
+    then have "signum (sum_list (map (\<lambda>i. vote_Spectre G i b c) 
+      (sorted_list_of_set (future_nodes G a)))) \<in> {0,1}" unfolding signum.simps
       by simp 
     then show ?thesis using four by simp 
   qed 
@@ -120,7 +120,7 @@ proof -
   have "(vote_Spectre G wit a b) \<in> set the_map" 
     unfolding the_map_in set_map 
     using B.blockDAG_axioms fin_digraph.finite_verts 
-      subs sorted_list_of_set(1) wit_in image_iff
+      subs(3) sorted_list_of_set(1) wit_in image_iff
     by metis 
   then have exune: "\<exists>x \<in> set the_map. x \<noteq> 0"
     using wit_vote by blast 
@@ -154,11 +154,11 @@ lemma "Order_Preserving SPECTRE"
   using SPECTRE_Preserving by auto 
 
 lemma vote_Spectre_antisymmetric: 
-  shows "b \<noteq> c \<Longrightarrow> vote_Spectre V a b c = - (vote_Spectre V a c b)"
-proof(induction V a b c rule: vote_Spectre.induct)
-  case (1 V a b c)
-  show "vote_Spectre V a b c = - vote_Spectre V a c b"
-  proof(cases a b c V rule:Spectre_casesAlt)
+  shows "b \<noteq> c \<Longrightarrow> vote_Spectre G a b c = - (vote_Spectre G a c b)"
+proof(induction G a b c rule: vote_Spectre.induct)
+  case (1 G a b c)
+  show "vote_Spectre G a b c = - vote_Spectre G a c b"
+  proof(cases a b c G rule:Spectre_casesAlt)
     case no_bD
     then show ?thesis by fastforce
   next
@@ -172,42 +172,42 @@ proof(induction V a b c rule: vote_Spectre.induct)
     then show ?thesis by fastforce
   next
     case three
-    then have ff: "vote_Spectre V a b c = tie_break_int b c (signum (sum_list (map (\<lambda>i.
- (vote_Spectre (reduce_past V a) i b c)) (sorted_list_of_set (past_nodes V a)))))"
+    then have ff: "vote_Spectre G a b c = tie_break_int b c (signum (sum_list (map (\<lambda>i.
+ (vote_Spectre (reduce_past G a) i b c)) (sorted_list_of_set (past_nodes G a)))))"
       using vote_Spectre.simps 
       by (metis (mono_tags, lifting)) 
-    have ff1: "vote_Spectre V a c b = tie_break_int c b (signum (sum_list (map (\<lambda>i.
-      (vote_Spectre (reduce_past V a) i c b)) (sorted_list_of_set (past_nodes V a)))))"
+    have ff1: "vote_Spectre G a c b = tie_break_int c b (signum (sum_list (map (\<lambda>i.
+      (vote_Spectre (reduce_past G a) i c b)) (sorted_list_of_set (past_nodes G a)))))"
       using vote_Spectre.simps three by fastforce 
-    then have ff2: "vote_Spectre V a c b = tie_break_int c b (signum (sum_list (map (\<lambda>i.
-    (- vote_Spectre (reduce_past V a) i b c)) (sorted_list_of_set (past_nodes V a)))))" 
+    then have ff2: "vote_Spectre G a c b = tie_break_int c b (signum (sum_list (map (\<lambda>i.
+    (- vote_Spectre (reduce_past G a) i b c)) (sorted_list_of_set (past_nodes G a)))))" 
       using three 1 map_eq_conv ff
       by (smt (verit, best))   
-    have "(map (\<lambda>i. - vote_Spectre (reduce_past V a) i b c) (sorted_list_of_set (past_nodes V a)))
-     = (map uminus (map (\<lambda>i. vote_Spectre (reduce_past V a) i b c)
-       (sorted_list_of_set (past_nodes V a))))" 
+    have "(map (\<lambda>i. - vote_Spectre (reduce_past G a) i b c) (sorted_list_of_set (past_nodes G a)))
+     = (map uminus (map (\<lambda>i. vote_Spectre (reduce_past G a) i b c)
+       (sorted_list_of_set (past_nodes G a))))" 
       using map_map by auto       
-    then have "vote_Spectre V a c b = - (tie_break_int b c (signum (sum_list (map (\<lambda>i.
-    (vote_Spectre (reduce_past V a) i b c)) (sorted_list_of_set (past_nodes V a))))))" 
+    then have "vote_Spectre G a c b = - (tie_break_int b c (signum (sum_list (map (\<lambda>i.
+    (vote_Spectre (reduce_past G a) i b c)) (sorted_list_of_set (past_nodes G a))))))" 
       using  antisymmetric_sumlist 1 ff2 antisymmetric_signum antisymmetric_tie_break
       by (metis verit_minus_simplify(4)) 
     then show ?thesis using  ff
       by presburger 
   next
     case four
-    then have ff: "vote_Spectre V a b c = signum (sum_list (map (\<lambda>i.
-   (vote_Spectre V i b c)) (sorted_list_of_set (future_nodes V a))))"
+    then have ff: "vote_Spectre G a b c = signum (sum_list (map (\<lambda>i.
+   (vote_Spectre G i b c)) (sorted_list_of_set (future_nodes G a))))"
       using vote_Spectre.simps
       by (metis (mono_tags, lifting)) 
-    then have ff2: "vote_Spectre V a c b =  signum (sum_list (map (\<lambda>i.
-    (- vote_Spectre V i b c)) (sorted_list_of_set (future_nodes V a))))" 
+    then have ff2: "vote_Spectre G a c b =  signum (sum_list (map (\<lambda>i.
+    (- vote_Spectre G i b c)) (sorted_list_of_set (future_nodes G a))))" 
       using four 1 vote_Spectre.simps map_eq_conv
       by (smt (z3)) 
-    have "(map (\<lambda>i. - vote_Spectre V i b c) (sorted_list_of_set (future_nodes V a)))
-     = (map uminus (map (\<lambda>i. vote_Spectre V i b c) (sorted_list_of_set (future_nodes V a))))" 
+    have "(map (\<lambda>i. - vote_Spectre G i b c) (sorted_list_of_set (future_nodes G a)))
+     = (map uminus (map (\<lambda>i. vote_Spectre G i b c) (sorted_list_of_set (future_nodes G a))))" 
       using map_map by auto       
-    then have "vote_Spectre V a c b = - ( signum (sum_list (map (\<lambda>i.
-    (vote_Spectre V i b c)) (sorted_list_of_set (future_nodes V a)))))" 
+    then have "vote_Spectre G a c b = - ( signum (sum_list (map (\<lambda>i.
+    (vote_Spectre G i b c)) (sorted_list_of_set (future_nodes G a)))))" 
       using  antisymmetric_sumlist 1 ff2 antisymmetric_signum 
       by (metis verit_minus_simplify(4)) 
     then show ?thesis using ff
@@ -217,55 +217,55 @@ qed
 
 
 lemma vote_Spectre_reflexive:
-  assumes "blockDAG V"
-    and "a \<in> verts V"
-  shows "\<forall>b \<in> verts V. vote_Spectre V b a a = 1 " using vote_Spectre.simps assms by auto 
+  assumes "blockDAG G"
+    and "a \<in> verts G"
+  shows "\<forall>b \<in> verts G. vote_Spectre G b a a = 1 " using vote_Spectre.simps assms by auto 
 
 lemma Spectre_Order_reflexive:
-  assumes "blockDAG V"
-    and "a \<in> verts V" 
-  shows "Spectre_Order V a a" 
+  assumes "blockDAG G"
+    and "a \<in> verts G" 
+  shows "Spectre_Order G a a" 
   unfolding Spectre_Order_def 
 proof -   
-  obtain l where l_def: "l = (map (\<lambda>i. vote_Spectre V i a a) (sorted_list_of_set (verts V)))"
+  obtain l where l_def: "l = (map (\<lambda>i. vote_Spectre G i a a) (sorted_list_of_set (verts G)))"
     by auto
-  have only_one: "l = (map (\<lambda>i.1) (sorted_list_of_set (verts V)))"
+  have only_one: "l = (map (\<lambda>i.1) (sorted_list_of_set (verts G)))"
     using l_def vote_Spectre_reflexive assms sorted_list_of_set(1)
     by (simp add: fin_digraph.finite_verts subs)
   have ne: "l \<noteq> []"
     using  blockDAG.no_empty_blockDAG length_map
     by (metis assms(1) length_sorted_list_of_set less_numeral_extra(3) list.size(3) l_def)
-  have "sum_list l = card (verts V)" using ne only_one sum_list_map_eq_sum_count
+  have "sum_list l = card (verts G)" using ne only_one sum_list_map_eq_sum_count
     by (simp add: sum_list_triv)
   then have "sum_list l > 0" using blockDAG.no_empty_blockDAG assms(1) by simp
   then show "tie_break_int a a
-    (signum (sum_list (map (\<lambda>i. vote_Spectre V i a a) (sorted_list_of_set (verts V))))) = 1"
+    (signum (sum_list (map (\<lambda>i. vote_Spectre G i a a) (sorted_list_of_set (verts G))))) = 1"
     using l_def ne  tie_break_int.simps
       list.exhaust verit_comp_simplify1(1) by auto
 qed
 
 
 lemma Spectre_Order_antisym: 
-  assumes "blockDAG V"
-    and "a \<in> verts V" 
-    and "b \<in> verts V" 
+  assumes "blockDAG G"
+    and "a \<in> verts G" 
+    and "b \<in> verts G" 
     and "a \<noteq> b"
-  shows "Spectre_Order V a b = (\<not> (Spectre_Order V b a))"
+  shows "Spectre_Order G a b = (\<not> (Spectre_Order G b a))"
 proof -
-  obtain wit where wit_in: "vote_Spectre V wit a b \<noteq> 0 \<and> wit \<in> verts V" 
+  obtain wit where wit_in: "vote_Spectre G wit a b \<noteq> 0 \<and> wit \<in> verts G" 
     using  vote_Spectre_one_exists assms
     by blast 
-  obtain l where l_def: "l = (map (\<lambda>i. vote_Spectre V i a b) (sorted_list_of_set (verts V)))"
+  obtain l where l_def: "l = (map (\<lambda>i. vote_Spectre G i a b) (sorted_list_of_set (verts G)))"
     by auto
-  have "wit \<in>  set (sorted_list_of_set (verts V))" 
+  have "wit \<in>  set (sorted_list_of_set (verts G))" 
     using  wit_in sorted_list_of_set(1) 
       fin_digraph.finite_verts subs
     by (simp add: fin_digraph.finite_verts subs assms(1)) 
-  then have "vote_Spectre V wit a b \<in> set l" unfolding l_def
+  then have "vote_Spectre G wit a b \<in> set l" unfolding l_def
     by (metis (mono_tags, lifting) image_eqI list.set_map)
   then have dm: "tie_break_int a b (signum (sum_list l)) \<in> {-1,1}"
     by auto  
-  obtain l2 where l2_def: "l2 = (map (\<lambda>i. vote_Spectre V i b a) (sorted_list_of_set (verts V)))"
+  obtain l2 where l2_def: "l2 = (map (\<lambda>i. vote_Spectre G i b a) (sorted_list_of_set (verts G)))"
     by auto
   have minus: "l2 = map uminus l"
     unfolding l_def l2_def map_map
@@ -280,13 +280,13 @@ proof -
 qed  
 
 lemma Spectre_Order_total:
-  assumes "blockDAG V"
-    and "a \<in> verts V \<and> b \<in> verts V" 
-  shows "Spectre_Order V a b \<or> Spectre_Order V b a"
+  assumes "blockDAG G"
+    and "a \<in> verts G \<and> b \<in> verts G" 
+  shows "Spectre_Order G a b \<or> Spectre_Order G b a"
 proof safe
-  assume notB: " \<not> Spectre_Order V b a"
+  assume notB: " \<not> Spectre_Order G b a"
   consider (eq) "a = b"| (neq) "a \<noteq> b" by auto
-  then show "Spectre_Order V a b"
+  then show "Spectre_Order G a b"
   proof (cases)
     case eq
     then show ?thesis using Spectre_Order_reflexive assms by metis
