TopSortD.thy
@@ -1,0 +1,337 @@
+theory TopSort
+  imports DAGs Utils "HOL-Library.Comparator"
+begin
+
+
+text \<open>Function to sort a list $L$ under a graph G such if $a$ references $b$,
+$b$ precedes $a$ in the list\<close>
+
+
+fun top_insert:: "('a::linorder,'b) pre_digraph \<Rightarrow>'a list \<Rightarrow> 'a \<Rightarrow> 'a list"
+  where "top_insert G [] a = [a]"
+  | "top_insert G (b # L) a = (if (b \<rightarrow>\<^sup>+\<^bsub>G\<^esub> a) then  (a # ( b # L)) else (b # top_insert G L a))"
+
+fun top_sort:: "('a::linorder,'b) pre_digraph \<Rightarrow> 'a list \<Rightarrow> 'a list"
+  where "top_sort G []= [] "
+  | "top_sort G (a # L) =  top_insert G (top_sort G L) a"
+
+subsubsection \<open>Soundness of the topological sort algorithm\<close>
+lemma top_insert_set: "set (top_insert G L a) = set L \<union> {a}" 
+proof(induct L, simp_all, auto) qed 
+
+
+lemma top_sort_con: "set (top_sort G L) = set L"
+proof(induct L)
+  case Nil
+  then show ?case by auto
+next
+  case (Cons a L)
+  then show ?case using top_sort.simps(2) top_insert_set insert_is_Un list.simps(15) sup_commute
+    by (metis) 
+qed
+
+
+lemma top_insert_len: "length (top_insert G L a) = Suc (length L)"
+proof(induct L)
+  case Nil
+  then show ?case by auto
+next
+  case (Cons a L)
+  then show ?case using top_insert.simps(2) by auto
+qed
+
+lemma top_insert_not_nil: "top_insert G L a \<noteq> []"
+proof(induct L, auto) qed
+
+
+lemma top_sort_len: "length (top_sort G L) = length L"
+proof(induct L, simp)
+  case (Cons a L)
+  then have "length (a#L) = Suc (length L)" by auto
+  then show ?case using
+      top_insert_len top_sort.simps(2) Cons
+    by (simp add: top_insert_len)  
+qed
+
+
+lemma top_sort_nil: "top_sort G L = [] \<longleftrightarrow> L = []" 
+proof(auto, induct L, auto simp: top_insert_not_nil) qed
+
+lemma top_insert_mono:
+  assumes "(y, x) \<in> list_to_rel ls"
+  shows "(y, x) \<in> list_to_rel (top_insert G ls l)"
+  using assms 
+proof(induct ls, simp)
+  case (Cons a ls)
+  consider (rec) "a \<rightarrow>\<^sup>+\<^bsub>G\<^esub> l" | (nrec) "\<not> a \<rightarrow>\<^sup>+\<^bsub>G\<^esub> l" by auto
+  then show ?case 
+  proof(cases)
+    case rec
+    then have sinse: "(top_insert G (a # ls) l)  = l # a # ls"
+      unfolding top_insert.simps by simp
+    show ?thesis unfolding sinse list_to_rel.simps  using Cons
+      by auto
+  next
+    case nrec
+    then have sinse: "(top_insert G (a # ls) l)  = a # top_insert G ls l"
+      unfolding top_insert.simps by simp
+    consider (ya) "y = a" | (yan) "(y, x) \<in> list_to_rel ls" using Cons by auto
+    then show ?thesis proof(cases)
+      case ya
+      then show ?thesis unfolding sinse list_to_rel.simps
+        by (metis Cons.prems SigmaI UnI1 top_insert_set insertCI list_to_rel_in sinse) 
+    next
+      case yan
+      then show ?thesis using Cons unfolding sinse list_to_rel.simps by auto 
+    qed
+  qed
+qed
+
+lemma top_insert_cases:
+  assumes "(y, x) \<in> list_to_rel (top_insert G ls l)"
+  shows  "(y, x) \<in> list_to_rel ls \<or> x = l \<or> y = l" 
+  using assms 
+proof(induct "(top_insert G ls l)" arbitrary: ls l, simp)
+  case (Cons a ls2)
+  consider "a # ls2 = l # ls" |  "a # ls2 = (hd ls) # top_insert G (tl ls) l" 
+    using Cons(2) top_insert.simps
+    by (metis list.sel(1) list.sel(3) top_insert.elims) 
+  then show ?case proof(cases)
+    case 1
+    then show ?thesis unfolding Cons(2) using Cons(3) list_to_rel_cases
+      by auto
+  next
+    case 2
+    then consider (ay) "a = y" |  (bb) "(y, x) \<in> list_to_rel ls2" 
+      using list_to_rel_elim Cons(2,3)
+      by metis 
+    then show ?thesis proof(cases)
+      case ay
+      then have "y = hd ls" using 2 by auto
+      moreover have "x \<in> set (a # ls2)" using list_to_rel_in Cons
+        by metis 
+      then show ?thesis  using  Cons
+        by (metis (no_types, lifting) "2" SigmaI UnI1 Un_iff ay calculation 
+    empty_iff empty_set list.inject list.sel(1) list.sel(2) list.set_intros(1) 
+    list.simps(15) list_to_rel.elims not_Cons_self2 set_ConsD  top_insert_set) 
+    next
+      case bb
+      then have "(y, x) \<in> list_to_rel (top_insert G (tl ls) l)"
+        using 2 by auto
+      then have "(y, x) \<in> list_to_rel (tl ls) \<or> x = l \<or> y = l"
+        using Cons 2
+        by blast 
+      then show ?thesis using list_to_rel_mono3 hd_Cons_tl list.sel(2)
+        by (metis) 
+    qed  
+  qed
+qed
+
+
+lemma top_insert_elims:
+  assumes "(y, x) \<notin> list_to_rel ls"
+  and "x \<noteq> l"
+  and "y \<noteq> l"
+  shows "(y, x) \<notin> list_to_rel (top_insert G ls l)"
+  using assms top_insert_cases by metis
+
+lemma top_sort_mono:
+  assumes "(y, x) \<in> list_to_rel (top_sort G ls)"
+  shows "(y, x) \<in> list_to_rel (top_sort G (l # ls))"
+  using assms 
+  by (simp add: top_insert_mono) 
+
+
+
+lemma top_sort_mono2:
+ "list_to_rel (top_sort G ls) \<subseteq>  list_to_rel (top_sort G (l # ls))"
+  using top_sort_mono
+  by (metis subrelI)
+
+lemma top_sort_one:
+  assumes "top_sort G L = [l]"
+  shows "L = [l]"
+proof -
+  have l_in: "l \<in> set L" using assms(1) top_sort_con
+    by (metis list.set_intros(1))   
+  have ll: "length L = length (top_sort G L) " using top_sort_len by metis
+  have "length L = 1" unfolding ll using assms by auto 
+  then show "L = [l]"  using l_in
+    by (metis append_butlast_last_id diff_is_0_eq'
+        le_numeral_extra(4) length_0_conv length_butlast
+        length_pos_if_in_set less_numeral_extra(3) self_append_conv2 set_ConsD) 
+qed
+
+lemma top_sort_cases:
+  assumes "(y, x) \<in> list_to_rel (top_sort G (l # ls))"
+  shows "(y, x) \<in> list_to_rel (top_sort G ls) \<or> y = l \<or> x = l" 
+  using assms
+proof(induct ls arbitrary: l, simp)
+  case (Cons a ls)
+  then show ?case 
+    unfolding top_sort.simps using top_insert_cases 
+    by metis 
+qed
+
+fun (in DAG) top_sorted :: "'a list \<Rightarrow> bool" where
+  "top_sorted [] = True" |
+  "top_sorted (x # ys) = ((\<forall>y \<in> set ys. \<not> x \<rightarrow>\<^sup>+\<^bsub>G\<^esub> y) \<and> top_sorted ys)"
+
+lemma (in DAG) top_sorted_sub:
+  assumes "S = drop k L"
+    and "top_sorted L"  
+  shows "top_sorted S"
+  using assms
+proof(induct k arbitrary: L S)
+  case 0
+  then show ?case by auto
+next
+  case (Suc k)
+  then show ?case unfolding drop_Suc using top_sorted.simps
+    by (metis Suc.prems(1) drop_Nil list.sel(3) top_sorted.elims(2)) 
+qed
+
+
+lemma top_insert_part_ord:
+  assumes "DAG G"
+    and "DAG.top_sorted G L"
+  shows "DAG.top_sorted G (top_insert G L a)" 
+  using assms 
+proof(induct L)
+  case Nil
+  then show ?case  
+    by (simp add: DAG.top_sorted.simps)  
+next
+  case (Cons b list)
+  consider (re) "b \<rightarrow>\<^sup>+\<^bsub>G\<^esub> a" | (nre) "\<not> b \<rightarrow>\<^sup>+\<^bsub>G\<^esub> a " by auto
+  then show ?case proof(cases)
+    case re
+    have "(\<forall>y\<in>set (b # list). \<not> a \<rightarrow>\<^sup>+\<^bsub>G\<^esub> y )" 
+    proof(rule ccontr)
+      assume "\<not> (\<forall>y\<in>set (b # list). \<not> a \<rightarrow>\<^sup>+\<^bsub>G\<^esub> y)"
+      then obtain wit where wit_in: "wit \<in> set  (b # list) \<and> a \<rightarrow>\<^sup>+\<^bsub>G\<^esub> wit" by auto
+      then have "b \<rightarrow>\<^sup>+\<^bsub>G\<^esub> wit" using re
+        by auto 
+      then have "\<not> DAG.top_sorted G  (b # list)"
+        using wit_in using DAG.top_sorted.simps(2) Cons(2)
+        by (metis DAG.cycle_free set_ConsD) 
+      then show "False" using Cons by auto 
+    qed
+    then show ?thesis using assms(1) DAG.top_sorted.simps Cons
+      by (simp add: DAG.top_sorted.simps(2) re) 
+  next
+    case nre
+    have "DAG.top_sorted G list" using Cons(2,3)
+      by (metis DAG.top_sorted.simps(2)) 
+    then have "DAG.top_sorted G (top_insert G list a)" 
+      using  Cons(1,2) by auto
+    moreover have "(\<forall>y\<in>set (top_insert G list a). \<not> b \<rightarrow>\<^sup>+\<^bsub>G\<^esub> y )" using top_insert_set 
+        Cons DAG.top_sorted.simps(2) nre
+      by (metis Un_iff empty_iff empty_set list.simps(15) set_ConsD)  
+    ultimately show ?thesis using Cons(2)
+      by (simp add: DAG.top_sorted.simps(2) nre)  
+  qed 
+qed
+
+
+lemma top_sort_sorted:
+  assumes "DAG G"
+  shows "DAG.top_sorted G (top_sort G L)" 
+  using assms 
+proof(induct L)
+  case Nil
+  then show ?case
+    by (simp add: DAG.top_sorted.simps(1)) 
+  case (Cons a L)
+  then show ?case unfolding top_sort.simps using top_insert_part_ord by auto
+qed
+
+lemma top_sorted_rel: 
+  assumes "DAG G"
+    and "y \<rightarrow>\<^sup>+\<^bsub>G\<^esub> x"
+    and "x \<in> set L"
+    and "y \<in> set L"
+    and "DAG.top_sorted G L"
+  shows "(x,y) \<in> list_to_rel L"
+  using assms
+proof(induct L, simp)
+  have une:"x \<noteq> y" using assms
+    by (metis DAG.cycle_free) 
+  case (Cons a L)
+  then consider "x = a \<and> y \<in> set (a # L)" | "y = a \<and> x \<in> set L" | "x \<in> set L \<and> y \<in> set L"
+    using une by auto
+  then show ?case proof(cases)
+    case 1
+    then show ?thesis unfolding list_to_rel.simps by auto
+  next
+    case 2
+    then have "\<not> DAG.top_sorted G (a # L)"
+      using assms DAG.top_sorted.simps(2)
+      by fastforce  
+    then show ?thesis using Cons by auto
+  next
+    case 3
+    then show ?thesis unfolding list_to_rel.simps using Cons DAG.top_sorted.simps(2) Un_iff
+      by metis  
+  qed
+qed
+
+lemma top_sort_rel: 
+  assumes "DAG G"
+    and "y \<rightarrow>\<^sup>+\<^bsub>G\<^esub> x"
+    and "x \<in> set L"
+    and "y \<in> set L"
+  shows "(x,y) \<in> list_to_rel (top_sort G L)"
+  using assms top_sort_sorted top_sorted_rel top_sort_con
+  by metis  
+
+lemma top_sorted_rel2: 
+  assumes "DAG G"
+    and "(x,y) \<in> list_to_rel L"
+    and "x \<in> set L"
+    and "y \<in> set L"
+    and "DAG.top_sorted G L"
+  shows "\<not> x \<rightarrow>\<^sup>+\<^bsub>G\<^esub> y"
+proof(rule ccontr)
+  assume " \<not> (x, y) \<notin> (arcs_ends G)\<^sup>+"
+  then show "False"
+    using assms(2,3,4,5)
+  proof(induct L, simp)
+   interpret D: DAG G using assms(1) by auto
+   case (Cons a L)
+   then consider "x = a \<and> y = a"
+     |"x = a \<and> y \<in> set L" | "y = a \<and> x \<in> set L" | "x \<in> set L \<and> y \<in> set L"
+    using Cons by auto
+    then show ?case proof(cases)
+      case 1
+      then show ?thesis using Cons
+        using D.cycle_free by blast 
+    next
+      case 2
+      then show ?thesis
+        using Cons.prems(1) Cons.prems(5) D.top_sorted.simps(2) by blast 
+    next
+      case 3
+      then show ?thesis
+        by (metis Cons.hyps Cons.prems(1) Cons.prems(2)
+            Cons.prems(5) D.top_sorted.simps(2) list_to_rel_elim list_to_rel_in) 
+    next
+      case 4
+      then show ?thesis
+        using Cons.hyps Cons.prems(1) Cons.prems(2) Cons.prems(5) by auto 
+    qed
+  qed
+qed
+
+
+lemma top_sort_rel2: 
+  assumes "DAG G"
+    and "(x,y) \<in> list_to_rel (top_sort G L)"
+    and "x \<in> set L"
+    and "y \<in> set L"
+  shows "\<not> x \<rightarrow>\<^sup>+\<^bsub>G\<^esub> y"
+  using assms top_sort_sorted top_sorted_rel2 top_sort_con by metis
+ 
+
+
+end
